proofs/specs/MLDSA.ec
@@ -3,7 +3,7 @@ from Jasmin require import JByte_array JWord.
 
 require import Parameters GFq Rq VecMat Conversion Serialization Symmetric Sampling.
 import PolyLVec PolyKVec PolyMat.
-import CDR Round Zq PolyReduceZq BigZMod MLDSAParams.
+import Round ZModQ ZpC Zp Zq PolyReduceZq MLDSAParams.
 
 type Leakage = [
    | RO of bool list
