proofs/x86-64/avx2/ml_dsa_65/common/arithmetic/common_modular.ec
@@ -6,7 +6,7 @@ from JazzEC require import Ml_dsa_65_avx2 Mldsa_65_prelude.
 
 from Spec require import GFq Rq Parameters MLDSA_W32_Rep.
 
-import CDR Round Zq.
+import Round ZModQ ZpC Zp Zq.
 
 require import Array256.
 
