proofs/x86-64/avx2/ml_dsa_65/ml_dsa_65_avx2.ec
@@ -4340,7 +4340,8 @@ module M = {
     var w:W64.t;
     var t16:W64.t;
     var t8:W64.t;
-    if ((((aT < cUR) \/ ((cUR + 8) <= aT)) \/ ((lEN = 0) /\ (tRAIL = 0)))) {
+    if (((((lEN < 0) \/ (aT < cUR)) \/ ((cUR + 8) <= aT)) \/
+        ((lEN = 0) /\ (tRAIL = 0)))) {
       w <- (W64.of_int 0);
     } else {
       if ((8 <= lEN)) {
@@ -4407,7 +4408,8 @@ module M = {
     var w:W128.t;
     var t64_0:W64.t;
     var t64_1:W64.t;
-    if ((((aT < cUR) \/ ((cUR + 16) <= aT)) \/ ((lEN = 0) /\ (tRAIL = 0)))) {
+    if (((((lEN < 0) \/ (aT < cUR)) \/ ((cUR + 16) <= aT)) \/
+        ((lEN = 0) /\ (tRAIL = 0)))) {
       w <- (set0_128);
     } else {
       if ((16 <= lEN)) {
@@ -4441,7 +4443,8 @@ module M = {
     var w:W256.t;
     var t128_0:W128.t;
     var t128_1:W128.t;
-    if ((((aT < cUR) \/ ((cUR + 32) <= aT)) \/ ((lEN = 0) /\ (tRAIL = 0)))) {
+    if (((((lEN < 0) \/ (aT < cUR)) \/ ((cUR + 32) <= aT)) \/
+        ((lEN = 0) /\ (tRAIL = 0)))) {
       w <- (set0_256);
     } else {
       if (((aT = cUR) /\ (32 <= lEN))) {
@@ -4473,28 +4476,25 @@ module M = {
                                          cUR:int, aT:int) : int * int * int *
                                                             int * W256.t = {
     var w256:W256.t;
-    var aT8:int;
     var w:W64.t;
     var t128:W128.t;
-    if ((((aT < cUR) \/ ((cUR + 8) <= aT)) \/ ((lEN = 0) /\ (tRAIL = 0)))) {
+    if (((((lEN < 0) \/ (aT < cUR)) \/ ((cUR + 8) <= aT)) \/
+        ((lEN = 0) /\ (tRAIL = 0)))) {
       w256 <- (set0_256);
     } else {
       if ((8 <= lEN)) {
-        aT8 <- (aT - cUR);
         w256 <-
         (VPBROADCAST_4u64
         (get64_direct (WArray2.init8 (fun i => buf.[i])) (offset + dELTA)));
-        w256 <@ __SHLQ_256 (w256, aT8);
-        dELTA <- (dELTA + (8 - aT8));
-        lEN <- (lEN - (8 - aT8));
+        w256 <@ __SHLQ_256 (w256, (aT - cUR));
+        dELTA <- (dELTA + ((cUR + 8) - aT));
+        lEN <- (lEN - ((cUR + 8) - aT));
         aT <- (cUR + 8);
       } else {
-        aT8 <- (aT - cUR);
         (dELTA, lEN, tRAIL, aT, w) <@ a2____a_ilen_read_upto8_at (buf,
         offset, dELTA, lEN, tRAIL, cUR, aT);
         t128 <- (VMOV_64 w);
         w256 <- (VPBROADCAST_4u64 (truncateu64 t128));
-        w256 <@ __SHLQ_256 (w256, aT8);
       }
     }
     return (dELTA, lEN, tRAIL, aT, w256);
@@ -4798,7 +4798,8 @@ module M = {
     var w:W64.t;
     var t16:W64.t;
     var t8:W64.t;
-    if ((((aT < cUR) \/ ((cUR + 8) <= aT)) \/ ((lEN = 0) /\ (tRAIL = 0)))) {
+    if (((((lEN < 0) \/ (aT < cUR)) \/ ((cUR + 8) <= aT)) \/
+        ((lEN = 0) /\ (tRAIL = 0)))) {
       w <- (W64.of_int 0);
     } else {
       if ((8 <= lEN)) {
@@ -4867,7 +4868,8 @@ module M = {
     var w:W128.t;
     var t64_0:W64.t;
     var t64_1:W64.t;
-    if ((((aT < cUR) \/ ((cUR + 16) <= aT)) \/ ((lEN = 0) /\ (tRAIL = 0)))) {
+    if (((((lEN < 0) \/ (aT < cUR)) \/ ((cUR + 16) <= aT)) \/
+        ((lEN = 0) /\ (tRAIL = 0)))) {
       w <- (set0_128);
     } else {
       if ((16 <= lEN)) {
@@ -4901,7 +4903,8 @@ module M = {
     var w:W256.t;
     var t128_0:W128.t;
     var t128_1:W128.t;
-    if ((((aT < cUR) \/ ((cUR + 32) <= aT)) \/ ((lEN = 0) /\ (tRAIL = 0)))) {
+    if (((((lEN < 0) \/ (aT < cUR)) \/ ((cUR + 32) <= aT)) \/
+        ((lEN = 0) /\ (tRAIL = 0)))) {
       w <- (set0_256);
     } else {
       if (((aT = cUR) /\ (32 <= lEN))) {
@@ -4934,28 +4937,25 @@ module M = {
                                                              int * int *
                                                              W256.t = {
     var w256:W256.t;
-    var aT8:int;
     var w:W64.t;
     var t128:W128.t;
-    if ((((aT < cUR) \/ ((cUR + 8) <= aT)) \/ ((lEN = 0) /\ (tRAIL = 0)))) {
+    if (((((lEN < 0) \/ (aT < cUR)) \/ ((cUR + 8) <= aT)) \/
+        ((lEN = 0) /\ (tRAIL = 0)))) {
       w256 <- (set0_256);
     } else {
       if ((8 <= lEN)) {
-        aT8 <- (aT - cUR);
         w256 <-
         (VPBROADCAST_4u64
         (get64_direct (WArray32.init8 (fun i => buf.[i])) (offset + dELTA)));
-        w256 <@ __SHLQ_256 (w256, aT8);
-        dELTA <- (dELTA + (8 - aT8));
-        lEN <- (lEN - (8 - aT8));
+        w256 <@ __SHLQ_256 (w256, (aT - cUR));
+        dELTA <- (dELTA + ((cUR + 8) - aT));
+        lEN <- (lEN - ((cUR + 8) - aT));
         aT <- (cUR + 8);
       } else {
-        aT8 <- (aT - cUR);
         (dELTA, lEN, tRAIL, aT, w) <@ a32____a_ilen_read_upto8_at (buf,
         offset, dELTA, lEN, tRAIL, cUR, aT);
         t128 <- (VMOV_64 w);
         w256 <- (VPBROADCAST_4u64 (truncateu64 t128));
-        w256 <@ __SHLQ_256 (w256, aT8);
       }
     }
     return (dELTA, lEN, tRAIL, aT, w256);
@@ -5161,7 +5161,8 @@ module M = {
     var w:W64.t;
     var t16:W64.t;
     var t8:W64.t;
-    if ((((aT < cUR) \/ ((cUR + 8) <= aT)) \/ ((lEN = 0) /\ (tRAIL = 0)))) {
+    if (((((lEN < 0) \/ (aT < cUR)) \/ ((cUR + 8) <= aT)) \/
+        ((lEN = 0) /\ (tRAIL = 0)))) {
       w <- (W64.of_int 0);
     } else {
       if ((8 <= lEN)) {
@@ -5230,7 +5231,8 @@ module M = {
     var w:W128.t;
     var t64_0:W64.t;
     var t64_1:W64.t;
-    if ((((aT < cUR) \/ ((cUR + 16) <= aT)) \/ ((lEN = 0) /\ (tRAIL = 0)))) {
+    if (((((lEN < 0) \/ (aT < cUR)) \/ ((cUR + 16) <= aT)) \/
+        ((lEN = 0) /\ (tRAIL = 0)))) {
       w <- (set0_128);
     } else {
       if ((16 <= lEN)) {
@@ -5264,7 +5266,8 @@ module M = {
     var w:W256.t;
     var t128_0:W128.t;
     var t128_1:W128.t;
-    if ((((aT < cUR) \/ ((cUR + 32) <= aT)) \/ ((lEN = 0) /\ (tRAIL = 0)))) {
+    if (((((lEN < 0) \/ (aT < cUR)) \/ ((cUR + 32) <= aT)) \/
+        ((lEN = 0) /\ (tRAIL = 0)))) {
       w <- (set0_256);
     } else {
       if (((aT = cUR) /\ (32 <= lEN))) {
@@ -5297,28 +5300,25 @@ module M = {
                                                              int * int *
                                                              W256.t = {
     var w256:W256.t;
-    var aT8:int;
     var w:W64.t;
     var t128:W128.t;
-    if ((((aT < cUR) \/ ((cUR + 8) <= aT)) \/ ((lEN = 0) /\ (tRAIL = 0)))) {
+    if (((((lEN < 0) \/ (aT < cUR)) \/ ((cUR + 8) <= aT)) \/
+        ((lEN = 0) /\ (tRAIL = 0)))) {
       w256 <- (set0_256);
     } else {
       if ((8 <= lEN)) {
-        aT8 <- (aT - cUR);
         w256 <-
         (VPBROADCAST_4u64
         (get64_direct (WArray64.init8 (fun i => buf.[i])) (offset + dELTA)));
-        w256 <@ __SHLQ_256 (w256, aT8);
-        dELTA <- (dELTA + (8 - aT8));
-        lEN <- (lEN - (8 - aT8));
+        w256 <@ __SHLQ_256 (w256, (aT - cUR));
+        dELTA <- (dELTA + ((cUR + 8) - aT));
+        lEN <- (lEN - ((cUR + 8) - aT));
         aT <- (cUR + 8);
       } else {
-        aT8 <- (aT - cUR);
         (dELTA, lEN, tRAIL, aT, w) <@ a64____a_ilen_read_upto8_at (buf,
         offset, dELTA, lEN, tRAIL, cUR, aT);
         t128 <- (VMOV_64 w);
         w256 <- (VPBROADCAST_4u64 (truncateu64 t128));
-        w256 <@ __SHLQ_256 (w256, aT8);
       }
     }
     return (dELTA, lEN, tRAIL, aT, w256);
@@ -5404,7 +5404,7 @@ module M = {
         } else {
           
         }
-        t64 <- (truncateu64 w);
+        t64 <- (MOVV_64 (truncateu64 w));
         (buf, dELTA, lEN) <@ a64____a_ilen_write_upto8 (buf, offset, 
         dELTA, lEN, t64);
       }
@@ -5618,8 +5618,8 @@ module M = {
   proc a64____dumpstate_avx2 (buf:W8.t Array64.t, offset:int, _LEN:int,
                               st:W256.t Array7.t) : W8.t Array64.t * int = {
     var dELTA:int;
-    var t128_0:W128.t;
     var t128_1:W128.t;
+    var t128_0:W128.t;
     var t:W64.t;
     var t256_0:W256.t;
     var t256_1:W256.t;
@@ -5639,9 +5639,9 @@ module M = {
     (buf, dELTA, _LEN) <@ a64____a_ilen_write_upto32 (buf, offset, dELTA,
     _LEN, st.[1]);
     if ((0 < _LEN)) {
-      t128_0 <- (truncateu128 st.[2]);
       t128_1 <- (VEXTRACTI128 st.[2] (W8.of_int 1));
-      t <- (truncateu64 t128_1);
+      t128_0 <- (truncateu128 st.[2]);
+      t <- (MOVV_64 (truncateu64 t128_1));
       (buf, dELTA, _LEN) <@ a64____a_ilen_write_upto8 (buf, offset, dELTA,
       _LEN, t);
       t128_1 <- (VPUNPCKH_2u64 t128_1 t128_1);
@@ -5724,7 +5724,7 @@ module M = {
         (buf, dELTA, _LEN) <@ a64____a_ilen_write_upto32 (buf, offset, 
         dELTA, _LEN, t256_4);
         if ((0 < _LEN)) {
-          t <- (truncateu64 t128_0);
+          t <- (MOVV_64 (truncateu64 t128_0));
           (buf, dELTA, _LEN) <@ a64____a_ilen_write_upto8 (buf, offset,
           dELTA, _LEN, t);
           t128_0 <- (VPUNPCKH_2u64 t128_0 t128_0);
@@ -5753,7 +5753,7 @@ module M = {
           
         }
         if ((0 < _LEN)) {
-          t <- (truncateu64 t128_1);
+          t <- (MOVV_64 (truncateu64 t128_1));
           (buf, dELTA, _LEN) <@ a64____a_ilen_write_upto8 (buf, offset,
           dELTA, _LEN, t);
         } else {
@@ -5781,7 +5781,7 @@ module M = {
           
         }
         if ((0 < _LEN)) {
-          t <- (truncateu64 t128_0);
+          t <- (MOVV_64 (truncateu64 t128_0));
           (buf, dELTA, _LEN) <@ a64____a_ilen_write_upto8 (buf, offset,
           dELTA, _LEN, t);
         } else {
@@ -6200,7 +6200,8 @@ module M = {
     var w:W64.t;
     var t16:W64.t;
     var t8:W64.t;
-    if ((((aT < cUR) \/ ((cUR + 8) <= aT)) \/ ((lEN = 0) /\ (tRAIL = 0)))) {
+    if (((((lEN < 0) \/ (aT < cUR)) \/ ((cUR + 8) <= aT)) \/
+        ((lEN = 0) /\ (tRAIL = 0)))) {
       w <- (W64.of_int 0);
     } else {
       if ((8 <= lEN)) {
@@ -6271,7 +6272,8 @@ module M = {
     var w:W128.t;
     var t64_0:W64.t;
     var t64_1:W64.t;
-    if ((((aT < cUR) \/ ((cUR + 16) <= aT)) \/ ((lEN = 0) /\ (tRAIL = 0)))) {
+    if (((((lEN < 0) \/ (aT < cUR)) \/ ((cUR + 16) <= aT)) \/
+        ((lEN = 0) /\ (tRAIL = 0)))) {
       w <- (set0_128);
     } else {
       if ((16 <= lEN)) {
@@ -6306,7 +6308,8 @@ module M = {
     var w:W256.t;
     var t128_0:W128.t;
     var t128_1:W128.t;
-    if ((((aT < cUR) \/ ((cUR + 32) <= aT)) \/ ((lEN = 0) /\ (tRAIL = 0)))) {
+    if (((((lEN < 0) \/ (aT < cUR)) \/ ((cUR + 32) <= aT)) \/
+        ((lEN = 0) /\ (tRAIL = 0)))) {
       w <- (set0_256);
     } else {
       if (((aT = cUR) /\ (32 <= lEN))) {
@@ -6339,28 +6342,25 @@ module M = {
                                                               int * int *
                                                               W256.t = {
     var w256:W256.t;
-    var aT8:int;
     var w:W64.t;
     var t128:W128.t;
-    if ((((aT < cUR) \/ ((cUR + 8) <= aT)) \/ ((lEN = 0) /\ (tRAIL = 0)))) {
+    if (((((lEN < 0) \/ (aT < cUR)) \/ ((cUR + 8) <= aT)) \/
+        ((lEN = 0) /\ (tRAIL = 0)))) {
       w256 <- (set0_256);
     } else {
       if ((8 <= lEN)) {
-        aT8 <- (aT - cUR);
         w256 <-
         (VPBROADCAST_4u64
         (get64_direct (WArray128.init8 (fun i => buf.[i])) (offset + dELTA)));
-        w256 <@ __SHLQ_256 (w256, aT8);
-        dELTA <- (dELTA + (8 - aT8));
-        lEN <- (lEN - (8 - aT8));
+        w256 <@ __SHLQ_256 (w256, (aT - cUR));
+        dELTA <- (dELTA + ((cUR + 8) - aT));
+        lEN <- (lEN - ((cUR + 8) - aT));
         aT <- (cUR + 8);
       } else {
-        aT8 <- (aT - cUR);
         (dELTA, lEN, tRAIL, aT, w) <@ a128____a_ilen_read_upto8_at (buf,
         offset, dELTA, lEN, tRAIL, cUR, aT);
         t128 <- (VMOV_64 w);
         w256 <- (VPBROADCAST_4u64 (truncateu64 t128));
-        w256 <@ __SHLQ_256 (w256, aT8);
       }
     }
     return (dELTA, lEN, tRAIL, aT, w256);
@@ -6446,7 +6446,7 @@ module M = {
         } else {
           
         }
-        t64 <- (truncateu64 w);
+        t64 <- (MOVV_64 (truncateu64 w));
         (buf, dELTA, lEN) <@ a128____a_ilen_write_upto8 (buf, offset, 
         dELTA, lEN, t64);
       }
@@ -6599,8 +6599,8 @@ module M = {
   proc a128____dumpstate_avx2 (buf:W8.t Array128.t, offset:int, _LEN:int,
                                st:W256.t Array7.t) : W8.t Array128.t * int = {
     var dELTA:int;
-    var t128_0:W128.t;
     var t128_1:W128.t;
+    var t128_0:W128.t;
     var t:W64.t;
     var t256_0:W256.t;
     var t256_1:W256.t;
@@ -6620,9 +6620,9 @@ module M = {
     (buf, dELTA, _LEN) <@ a128____a_ilen_write_upto32 (buf, offset, dELTA,
     _LEN, st.[1]);
     if ((0 < _LEN)) {
-      t128_0 <- (truncateu128 st.[2]);
       t128_1 <- (VEXTRACTI128 st.[2] (W8.of_int 1));
-      t <- (truncateu64 t128_1);
+      t128_0 <- (truncateu128 st.[2]);
+      t <- (MOVV_64 (truncateu64 t128_1));
       (buf, dELTA, _LEN) <@ a128____a_ilen_write_upto8 (buf, offset, 
       dELTA, _LEN, t);
       t128_1 <- (VPUNPCKH_2u64 t128_1 t128_1);
@@ -6705,7 +6705,7 @@ module M = {
         (buf, dELTA, _LEN) <@ a128____a_ilen_write_upto32 (buf, offset,
         dELTA, _LEN, t256_4);
         if ((0 < _LEN)) {
-          t <- (truncateu64 t128_0);
+          t <- (MOVV_64 (truncateu64 t128_0));
           (buf, dELTA, _LEN) <@ a128____a_ilen_write_upto8 (buf, offset,
           dELTA, _LEN, t);
           t128_0 <- (VPUNPCKH_2u64 t128_0 t128_0);
@@ -6734,7 +6734,7 @@ module M = {
           
         }
         if ((0 < _LEN)) {
-          t <- (truncateu64 t128_1);
+          t <- (MOVV_64 (truncateu64 t128_1));
           (buf, dELTA, _LEN) <@ a128____a_ilen_write_upto8 (buf, offset,
           dELTA, _LEN, t);
         } else {
@@ -6762,7 +6762,7 @@ module M = {
           
         }
         if ((0 < _LEN)) {
-          t <- (truncateu64 t128_0);
+          t <- (MOVV_64 (truncateu64 t128_0));
           (buf, dELTA, _LEN) <@ a128____a_ilen_write_upto8 (buf, offset,
           dELTA, _LEN, t);
         } else {
@@ -6879,7 +6879,7 @@ module M = {
         } else {
           
         }
-        t64 <- (truncateu64 w);
+        t64 <- (MOVV_64 (truncateu64 w));
         (buf, dELTA, lEN) <@ a136____a_ilen_write_upto8 (buf, offset, 
         dELTA, lEN, t64);
       }
@@ -6926,8 +6926,8 @@ module M = {
   proc a136____dumpstate_avx2 (buf:W8.t Array136.t, offset:int, _LEN:int,
                                st:W256.t Array7.t) : W8.t Array136.t * int = {
     var dELTA:int;
-    var t128_0:W128.t;
     var t128_1:W128.t;
+    var t128_0:W128.t;
     var t:W64.t;
     var t256_0:W256.t;
     var t256_1:W256.t;
@@ -6947,9 +6947,9 @@ module M = {
     (buf, dELTA, _LEN) <@ a136____a_ilen_write_upto32 (buf, offset, dELTA,
     _LEN, st.[1]);
     if ((0 < _LEN)) {
-      t128_0 <- (truncateu128 st.[2]);
       t128_1 <- (VEXTRACTI128 st.[2] (W8.of_int 1));
-      t <- (truncateu64 t128_1);
+      t128_0 <- (truncateu128 st.[2]);
+      t <- (MOVV_64 (truncateu64 t128_1));
       (buf, dELTA, _LEN) <@ a136____a_ilen_write_upto8 (buf, offset, 
       dELTA, _LEN, t);
       t128_1 <- (VPUNPCKH_2u64 t128_1 t128_1);
@@ -7032,7 +7032,7 @@ module M = {
         (buf, dELTA, _LEN) <@ a136____a_ilen_write_upto32 (buf, offset,
         dELTA, _LEN, t256_4);
         if ((0 < _LEN)) {
-          t <- (truncateu64 t128_0);
+          t <- (MOVV_64 (truncateu64 t128_0));
           (buf, dELTA, _LEN) <@ a136____a_ilen_write_upto8 (buf, offset,
           dELTA, _LEN, t);
           t128_0 <- (VPUNPCKH_2u64 t128_0 t128_0);
@@ -7061,7 +7061,7 @@ module M = {
           
         }
         if ((0 < _LEN)) {
-          t <- (truncateu64 t128_1);
+          t <- (MOVV_64 (truncateu64 t128_1));
           (buf, dELTA, _LEN) <@ a136____a_ilen_write_upto8 (buf, offset,
           dELTA, _LEN, t);
         } else {
@@ -7089,7 +7089,7 @@ module M = {
           
         }
         if ((0 < _LEN)) {
-          t <- (truncateu64 t128_0);
+          t <- (MOVV_64 (truncateu64 t128_0));
           (buf, dELTA, _LEN) <@ a136____a_ilen_write_upto8 (buf, offset,
           dELTA, _LEN, t);
         } else {
@@ -7432,7 +7432,8 @@ module M = {
     var w:W64.t;
     var t16:W64.t;
     var t8:W64.t;
-    if ((((aT < cUR) \/ ((cUR + 8) <= aT)) \/ ((lEN = 0) /\ (tRAIL = 0)))) {
+    if (((((lEN < 0) \/ (aT < cUR)) \/ ((cUR + 8) <= aT)) \/
+        ((lEN = 0) /\ (tRAIL = 0)))) {
       w <- (W64.of_int 0);
     } else {
       if ((8 <= lEN)) {
@@ -7503,7 +7504,8 @@ module M = {
     var w:W128.t;
     var t64_0:W64.t;
     var t64_1:W64.t;
-    if ((((aT < cUR) \/ ((cUR + 16) <= aT)) \/ ((lEN = 0) /\ (tRAIL = 0)))) {
+    if (((((lEN < 0) \/ (aT < cUR)) \/ ((cUR + 16) <= aT)) \/
+        ((lEN = 0) /\ (tRAIL = 0)))) {
       w <- (set0_128);
     } else {
       if ((16 <= lEN)) {
@@ -7539,7 +7541,8 @@ module M = {
     var w:W256.t;
     var t128_0:W128.t;
     var t128_1:W128.t;
-    if ((((aT < cUR) \/ ((cUR + 32) <= aT)) \/ ((lEN = 0) /\ (tRAIL = 0)))) {
+    if (((((lEN < 0) \/ (aT < cUR)) \/ ((cUR + 32) <= aT)) \/
+        ((lEN = 0) /\ (tRAIL = 0)))) {
       w <- (set0_256);
     } else {
       if (((aT = cUR) /\ (32 <= lEN))) {
@@ -7574,28 +7577,25 @@ module M = {
                                                                   int * int *
                                                                   W256.t = {
     var w256:W256.t;
-    var aT8:int;
     var w:W64.t;
     var t128:W128.t;
-    if ((((aT < cUR) \/ ((cUR + 8) <= aT)) \/ ((lEN = 0) /\ (tRAIL = 0)))) {
+    if (((((lEN < 0) \/ (aT < cUR)) \/ ((cUR + 8) <= aT)) \/
+        ((lEN = 0) /\ (tRAIL = 0)))) {
       w256 <- (set0_256);
     } else {
       if ((8 <= lEN)) {
-        aT8 <- (aT - cUR);
         w256 <-
         (VPBROADCAST_4u64
         (get64_direct (WArray48.init8 (fun i => buf.[i])) (offset + dELTA)));
-        w256 <@ __SHLQ_256 (w256, aT8);
-        dELTA <- (dELTA + (8 - aT8));
-        lEN <- (lEN - (8 - aT8));
+        w256 <@ __SHLQ_256 (w256, (aT - cUR));
+        dELTA <- (dELTA + ((cUR + 8) - aT));
+        lEN <- (lEN - ((cUR + 8) - aT));
         aT <- (cUR + 8);
       } else {
-        aT8 <- (aT - cUR);
         (dELTA, lEN, tRAIL, aT, w) <@ a_COMMITMENT_HASH____a_ilen_read_upto8_at (
         buf, offset, dELTA, lEN, tRAIL, cUR, aT);
         t128 <- (VMOV_64 w);
         w256 <- (VPBROADCAST_4u64 (truncateu64 t128));
-        w256 <@ __SHLQ_256 (w256, aT8);
       }
     }
     return (dELTA, lEN, tRAIL, aT, w256);
@@ -7683,7 +7683,7 @@ module M = {
         } else {
           
         }
-        t64 <- (truncateu64 w);
+        t64 <- (MOVV_64 (truncateu64 w));
         (buf, dELTA, lEN) <@ a_COMMITMENT_HASH____a_ilen_write_upto8 (
         buf, offset, dELTA, lEN, t64);
       }
@@ -7840,8 +7840,8 @@ module M = {
                                             _LEN:int, st:W256.t Array7.t) : 
   W8.t Array48.t * int = {
     var dELTA:int;
-    var t128_0:W128.t;
     var t128_1:W128.t;
+    var t128_0:W128.t;
     var t:W64.t;
     var t256_0:W256.t;
     var t256_1:W256.t;
@@ -7861,9 +7861,9 @@ module M = {
     (buf, dELTA, _LEN) <@ a_COMMITMENT_HASH____a_ilen_write_upto32 (buf,
     offset, dELTA, _LEN, st.[1]);
     if ((0 < _LEN)) {
-      t128_0 <- (truncateu128 st.[2]);
       t128_1 <- (VEXTRACTI128 st.[2] (W8.of_int 1));
-      t <- (truncateu64 t128_1);
+      t128_0 <- (truncateu128 st.[2]);
+      t <- (MOVV_64 (truncateu64 t128_1));
       (buf, dELTA, _LEN) <@ a_COMMITMENT_HASH____a_ilen_write_upto8 (
       buf, offset, dELTA, _LEN, t);
       t128_1 <- (VPUNPCKH_2u64 t128_1 t128_1);
@@ -7946,7 +7946,7 @@ module M = {
         (buf, dELTA, _LEN) <@ a_COMMITMENT_HASH____a_ilen_write_upto32 (
         buf, offset, dELTA, _LEN, t256_4);
         if ((0 < _LEN)) {
-          t <- (truncateu64 t128_0);
+          t <- (MOVV_64 (truncateu64 t128_0));
           (buf, dELTA, _LEN) <@ a_COMMITMENT_HASH____a_ilen_write_upto8 (
           buf, offset, dELTA, _LEN, t);
           t128_0 <- (VPUNPCKH_2u64 t128_0 t128_0);
@@ -7975,7 +7975,7 @@ module M = {
           
         }
         if ((0 < _LEN)) {
-          t <- (truncateu64 t128_1);
+          t <- (MOVV_64 (truncateu64 t128_1));
           (buf, dELTA, _LEN) <@ a_COMMITMENT_HASH____a_ilen_write_upto8 (
           buf, offset, dELTA, _LEN, t);
         } else {
@@ -8003,7 +8003,7 @@ module M = {
           
         }
         if ((0 < _LEN)) {
-          t <- (truncateu64 t128_0);
+          t <- (MOVV_64 (truncateu64 t128_0));
           (buf, dELTA, _LEN) <@ a_COMMITMENT_HASH____a_ilen_write_upto8 (
           buf, offset, dELTA, _LEN, t);
         } else {
@@ -8047,7 +8047,8 @@ module M = {
     var w:W64.t;
     var t16:W64.t;
     var t8:W64.t;
-    if ((((aT < cUR) \/ ((cUR + 8) <= aT)) \/ ((lEN = 0) /\ (tRAIL = 0)))) {
+    if (((((lEN < 0) \/ (aT < cUR)) \/ ((cUR + 8) <= aT)) \/
+        ((lEN = 0) /\ (tRAIL = 0)))) {
       w <- (W64.of_int 0);
     } else {
       if ((8 <= lEN)) {
@@ -8119,7 +8120,8 @@ module M = {
     var w:W128.t;
     var t64_0:W64.t;
     var t64_1:W64.t;
-    if ((((aT < cUR) \/ ((cUR + 16) <= aT)) \/ ((lEN = 0) /\ (tRAIL = 0)))) {
+    if (((((lEN < 0) \/ (aT < cUR)) \/ ((cUR + 16) <= aT)) \/
+        ((lEN = 0) /\ (tRAIL = 0)))) {
       w <- (set0_128);
     } else {
       if ((16 <= lEN)) {
@@ -8156,7 +8158,8 @@ module M = {
     var w:W256.t;
     var t128_0:W128.t;
     var t128_1:W128.t;
-    if ((((aT < cUR) \/ ((cUR + 32) <= aT)) \/ ((lEN = 0) /\ (tRAIL = 0)))) {
+    if (((((lEN < 0) \/ (aT < cUR)) \/ ((cUR + 32) <= aT)) \/
+        ((lEN = 0) /\ (tRAIL = 0)))) {
       w <- (set0_256);
     } else {
       if (((aT = cUR) /\ (32 <= lEN))) {
@@ -8194,29 +8197,26 @@ module M = {
                                                                    int *
                                                                    W256.t = {
     var w256:W256.t;
-    var aT8:int;
     var w:W64.t;
     var t128:W128.t;
-    if ((((aT < cUR) \/ ((cUR + 8) <= aT)) \/ ((lEN = 0) /\ (tRAIL = 0)))) {
+    if (((((lEN < 0) \/ (aT < cUR)) \/ ((cUR + 8) <= aT)) \/
+        ((lEN = 0) /\ (tRAIL = 0)))) {
       w256 <- (set0_256);
     } else {
       if ((8 <= lEN)) {
-        aT8 <- (aT - cUR);
         w256 <-
         (VPBROADCAST_4u64
         (get64_direct (WArray1952.init8 (fun i => buf.[i])) (offset + dELTA))
         );
-        w256 <@ __SHLQ_256 (w256, aT8);
-        dELTA <- (dELTA + (8 - aT8));
-        lEN <- (lEN - (8 - aT8));
+        w256 <@ __SHLQ_256 (w256, (aT - cUR));
+        dELTA <- (dELTA + ((cUR + 8) - aT));
+        lEN <- (lEN - ((cUR + 8) - aT));
         aT <- (cUR + 8);
       } else {
-        aT8 <- (aT - cUR);
         (dELTA, lEN, tRAIL, aT, w) <@ a_VERIFICATION_KEY____a_ilen_read_upto8_at (
         buf, offset, dELTA, lEN, tRAIL, cUR, aT);
         t128 <- (VMOV_64 w);
         w256 <- (VPBROADCAST_4u64 (truncateu64 t128));
-        w256 <@ __SHLQ_256 (w256, aT8);
       }
     }
     return (dELTA, lEN, tRAIL, aT, w256);
@@ -8337,7 +8337,8 @@ module M = {
     var w:W64.t;
     var t16:W64.t;
     var t8:W64.t;
-    if ((((aT < cUR) \/ ((cUR + 8) <= aT)) \/ ((lEN = 0) /\ (tRAIL = 0)))) {
+    if (((((lEN < 0) \/ (aT < cUR)) \/ ((cUR + 8) <= aT)) \/
+        ((lEN = 0) /\ (tRAIL = 0)))) {
       w <- (W64.of_int 0);
     } else {
       if ((8 <= lEN)) {
@@ -8409,7 +8410,8 @@ module M = {
     var w:W128.t;
     var t64_0:W64.t;
     var t64_1:W64.t;
-    if ((((aT < cUR) \/ ((cUR + 16) <= aT)) \/ ((lEN = 0) /\ (tRAIL = 0)))) {
+    if (((((lEN < 0) \/ (aT < cUR)) \/ ((cUR + 16) <= aT)) \/
+        ((lEN = 0) /\ (tRAIL = 0)))) {
       w <- (set0_128);
     } else {
       if ((16 <= lEN)) {
@@ -8445,7 +8447,8 @@ module M = {
     var w:W256.t;
     var t128_0:W128.t;
     var t128_1:W128.t;
-    if ((((aT < cUR) \/ ((cUR + 32) <= aT)) \/ ((lEN = 0) /\ (tRAIL = 0)))) {
+    if (((((lEN < 0) \/ (aT < cUR)) \/ ((cUR + 32) <= aT)) \/
+        ((lEN = 0) /\ (tRAIL = 0)))) {
       w <- (set0_256);
     } else {
       if (((aT = cUR) /\ (32 <= lEN))) {
@@ -8480,28 +8483,25 @@ module M = {
                                                            cUR:int, aT:int) : 
   int * int * int * int * W256.t = {
     var w256:W256.t;
-    var aT8:int;
     var w:W64.t;
     var t128:W128.t;
-    if ((((aT < cUR) \/ ((cUR + 8) <= aT)) \/ ((lEN = 0) /\ (tRAIL = 0)))) {
+    if (((((lEN < 0) \/ (aT < cUR)) \/ ((cUR + 8) <= aT)) \/
+        ((lEN = 0) /\ (tRAIL = 0)))) {
       w256 <- (set0_256);
     } else {
       if ((8 <= lEN)) {
-        aT8 <- (aT - cUR);
         w256 <-
         (VPBROADCAST_4u64
         (get64_direct (WArray768.init8 (fun i => buf.[i])) (offset + dELTA)));
-        w256 <@ __SHLQ_256 (w256, aT8);
-        dELTA <- (dELTA + (8 - aT8));
-        lEN <- (lEN - (8 - aT8));
+        w256 <@ __SHLQ_256 (w256, (aT - cUR));
+        dELTA <- (dELTA + ((cUR + 8) - aT));
+        lEN <- (lEN - ((cUR + 8) - aT));
         aT <- (cUR + 8);
       } else {
-        aT8 <- (aT - cUR);
         (dELTA, lEN, tRAIL, aT, w) <@ a_ENCODED_COMMITMENT____a_ilen_read_upto8_at (
         buf, offset, dELTA, lEN, tRAIL, cUR, aT);
         t128 <- (VMOV_64 w);
         w256 <- (VPBROADCAST_4u64 (truncateu64 t128));
-        w256 <@ __SHLQ_256 (w256, aT8);
       }
     }
     return (dELTA, lEN, tRAIL, aT, w256);
