proofs/x86-64/avx2/ml_dsa_65/sign.ec
@@ -12,7 +12,7 @@ from Spec require import GFq Rq Serialization Conversion Parameters VecMat
                          Symmetric Sampling MLDSA_W32_Rep MLDSA.
 
 import PolyLVec PolyKVec PolyMat.
-import CDR Round Zq PolyReduceZq BigZMod.
+import Round ZModQ ZpC Zp Zq PolyReduceZq.
 
 require import Array2 Array32 Array48 Array64 Array128 Array256
                Array416 Array640 Array768 Array1280 Array1536 Array2496
